generational/spec/GC.Gen.CheneyCorrectness.fsti
@@ -342,8 +342,9 @@ val chunked_cheney_gc_correct_after_preflight
        j < U64.v (GC.Spec.Object.getWosize hdr) /\
        U64.v field_addr == U64.v src + j * U64.v mword /\
        MH.read_word_in_major major field_addr == Some old /\
-       ~(is_minor_pointer (to_minor_offset old) /\
-         collect.cmc_fwd (to_minor_offset old) <> 0UL) ==>
+       (U64.v (GC.Spec.Object.getTag hdr) >= U64.v GC.Spec.Object.no_scan_tag \/
+        ~(is_minor_pointer (to_minor_offset old) /\
+          collect.cmc_fwd (to_minor_offset old) <> 0UL)) ==>
        MH.read_word_in_major collect.cmc_major field_addr == Some old) /\
       (forall (x: U64.t). Seq.mem x (minor_reachable minor roots) ==>
        collect.cmc_fwd x <> 0UL \/ minor_wosize minor x = 0)))
